Changed trans_alt, ssimalt, updated most lemmas in those files

theories/Eq/SSimAlt.v
@@ -13,57 +13,74 @@ From ITree Require Import Core.Subevent.
 From CTree Require Import
      CTree
      Utils
-     Eq
+     Eq.Equ
+     Eq.TransAlt
      Eq.Epsilon.
 
 From RelationAlgebra Require Export
-     rel srel.
+     monoid kat kat_tac rel srel.
 
 Import CoindNotations.
 Import CTree.
 Set Implicit Arguments.
 
 (* TODO: Decide where to set this *)
-Arguments trans : simpl never.
+Arguments trans_alt : simpl never.
 
 Ltac ssplit := split; [| split].
 
 Section StrongSimAlt.
 
-  Definition ss'_gen {E F C D : Type -> Type} {X Y : Type}
-    (L : rel (@label E) (@label F))
-    (R Reps : rel (ctree E C X) (ctree F D Y))
+  (* finition ss'_gen {E F C D : Type -> Type} {X : Type}
+    (L : rel (@label E X) (@label F X))
+    (R Reps : rel (ctree E C X) (ctree F D X))
     (t : ctree E C X) (u : ctree F D Y) :=
+
     (productive t ->
-     forall l t', trans l t t' ->
+    (* t and u step together under labels related by L, assuming 
+    t is "productive"; that is, not a Br *)
+      forall l t', trans l t t' ->
              exists l' u', trans l' u u' /\ R t' u' /\ L l l')
+    (* if t branches, u ϵ-steps to u'  *)
     /\ (forall Z (c : C Z) k,
           t ≅ Br c k ->
           forall x, exists u', epsilon u u' /\ Reps (k x) u')
     /\ (forall t',
           t ≅ Guard t' ->
           exists u', epsilon u u' /\ Reps t' u').
+ *)
+Locate dot. 
+  Definition ss'_gen {E F B : Type -> Type} {X : Type}
+    (L : rel (@label E X) (@label F X))
+    (R Reps : rel SS SS)
+    (t : SS) (u : SS) :=
 
-  #[global] Instance weq_ss'_gen {E F C D X Y} :
-    Proper (weq ==> weq) (@ss'_gen E F C D X Y).
+    (forall t' l, l <> ε -> trans_alt (B:=B) l t t'
+    -> exists l' u', ((trans_alt (B:=B) ε)^* ⋅ (trans_alt l')) u u' /\ R t' u' /\ L l l')
+    /\
+      (forall t', trans_alt (B:=B) ε t t' -> exists u', (trans_alt (B:=B) ε)^* u u' /\ Reps t' u').
+
+  #[global] Instance weq_ss'_gen {E F B X} :
+    Proper (weq ==> eq ==> weq) (@ss'_gen E F B X).
   Proof.
-    cbn. intros; split; (split; [| split]); intros.
-    all: try now (eapply H0 in H1 as (? & ? & ?); eauto).
-    all: apply H0 in H2 as (? & ? & ? & ? & ?); auto; edestruct H; eauto 6 with trans.
+    cbn. intros L L' HL R ? <- x y; split; intros (HA & HB); split; intros.
+    - destruct (HA _ _ H H0) as (l'' & u'' & Htrans & HR & HL').
+      do 2 esplit; split; [eassumption | split; [eassumption |]]; now apply HL.
+    - now apply HB in H.
+    - destruct (HA _ _ H H0) as (l'' & u'' & Htrans & HR & HL').
+      do 2 esplit; split; [eassumption | split; [eassumption |]]; now apply HL.
+    - now apply HB in H.
   Qed.
 
-  #[global] Instance ss'_gen_mon {E F C D : Type -> Type} {X Y : Type}
-    (L : rel (@label E) (@label F)) :
-    Proper (leq ==> leq ==> leq) (@ss'_gen E F C D X Y L).
+  #[global] Instance ss'_gen_mon {E F B X}
+    (L : rel (@label E X) (@label F X)) :
+    Proper (Coinduction.lattice.leq ==> Coinduction.lattice.leq ==> Coinduction.lattice.leq)
+     (@ss'_gen E F B X L).
   Proof.
-    cbn. intros.
-    destruct H1 as (? & ? & ?).
-    split; [| split].
-    - intros.
-      edestruct H1 as (? & ? & ? & ?); eauto.
-      eexists _, x2; intuition; eauto.
-    - intros. edestruct H2 as (? & ? & ?); eauto.
-    - intros. edestruct H3 as (? & ? & ?); eauto.
+    cbn. intros R R' HR Reps1 Reps2 HReps s1 s2 [Hl Hep]; split; intros.
+    - destruct (Hl _ _ H H0) as (l'' & u'' & Htrans & HRtu & HL').
+      do 2 esplit; split; [eassumption | split; [now apply HR | assumption]].
+    - apply Hep in H as (u' & Htrans & HRtu). exists u'; split; [assumption | now apply HReps].
   Qed.
 
 (*|
@@ -71,103 +88,121 @@ An alternative definition [ss'] of strong simulation.
 The simulation challenge does not involve an inductive transition relation,
 thus simplifying proofs.
 |*)
-  Program Definition ss' {E F C D : Type -> Type} {X Y : Type}
-    (L : rel (@label E) (@label F)) :
-    mon (ctree E C X -> ctree F D Y -> Prop) :=
+  Program Definition ss' {E F B : Type -> Type} {X : Type}
+    (L : rel (@label E X) (@label F X)) :
+    mon (SS -> SS -> Prop) :=
     {| body R t u :=
-      ss'_gen L R R t u
+      @ss'_gen E F B X L R R t u  
     |}.
-  Next Obligation.
-    epose proof (@ss'_gen_mon E F C D X Y). eapply H1.
+      Next Obligation.
+    epose proof (@ss'_gen_mon E F B X). eapply H1.
     3: apply H0.
     all: auto.
   Qed.
 
+
 End StrongSimAlt.
 
-Definition ssim' {E F C D X Y} L :=
-  (gfp (@ss' E F C D X Y L): hrel _ _).
+Definition ssim' {E F B X} L :=
+  (gfp (@ss' E F B X L): hrel _ _).
+
+Variant Seq_clos_body {E F B X} (R : rel (@S E B X) (@S F B X)) : rel (@S E B X) (@S F B X) :=
+  | Seq_clos_intro : forall t t' u' u
+                       (Seqt : t ⩸ t')
+                       (HR : R t' u')
+                       (Sequ : u' ⩸ u),
+      Seq_clos_body R t u.
+
+Program Definition Seq_clos {E F B X} : mon (rel (@S E B X) (@S F B X)) :=
+  {| body := @Seq_clos_body E F B X |}.
+Next Obligation.
+  match goal with h : Seq_clos_body _ _ _ |- _ => inv h end.
+  econstructor; eauto.
+Qed.
 
 Section ssim'_theory.
   Arguments label: clear implicits.
-  Context {E F C D: Type -> Type} {X Y: Type}
-          {L: rel (@label E) (@label F)}.
+  Context {E F B: Type -> Type} {X : Type}
+          {L: rel (@label E X) (@label F X)}.
 
 (*|
    Strong simulation up-to [equ] is valid
    ----------------------------------------
 |*)
-  #[global] Instance equ_ss'_gen_goal {R Reps} :
-    Proper (equ eq ==> equ eq ==> flip impl) (@ss'_gen E F C D X Y L R Reps).
+  #[global] Instance Seq_ss'_gen_goal {R Reps} :
+    Proper (Seq ==> Seq ==> flip impl) (@ss'_gen E F B X L R Reps).
   Proof.
-    split; [| split]; intros; subs; destruct H1 as (HA & HB & HC).
-    - apply HA in H3; auto.
-      destruct H3 as (? & ? & ? & ? & ?). eexists _, _. subs. etrans.
-    - symmetry in H. eapply HB in H. destruct H as (? & ? & ?).
-      eexists. subs. etrans.
-    - symmetry in H. eapply HC in H. destruct H as (? & ? & ?).
-      eexists. subs. etrans.
-   Qed.
-
-  #[global] Instance equ_ss'_gen_ctx {R Reps} :
-    Proper (equ eq ==> equ eq ==> impl) (@ss'_gen E F C D X Y L R Reps).
-  Proof.
-    do 4 red. intros. now rewrite <- H, <- H0.
+    intros t t' EQt u u' EQu (HA & HB); split.
+    - intros t'' l Hl TR. rewrite EQt in TR.
+      apply HA in TR as (l' & u'' & STEP & HRtu & HL); auto.
+      exists l', u''; split; [| split; assumption].
+      now rewrite EQu.
+    - intros t'' TR. rewrite EQt in TR.
+      apply HB in TR as (u'' & STEP & HRtu).
+      exists u''; split; [| assumption].
+      now rewrite EQu.
   Qed.
 
-  Lemma equ_clos_sst' {c: Chain (ss' L)}:
-    forall x y, @equ_clos E F C D X Y `c x y -> `c x y.
+  #[global] Instance Seq_ss'_gen_ctx {R Reps} :
+    Proper (Seq ==> Seq ==> impl) (@ss'_gen E F B X L R Reps).
+  Proof.
+    intros t t' EQt u u' EQu H. now rewrite <- EQt, <- EQu.
+  Qed.
+
+  Lemma Seq_clos_sst' {c: Chain (@ss' E F B X L)}:
+    forall x y, Seq_clos `c x y -> `c x y.
   Proof.
     apply tower.
-    - intros ? INC x y [x' y' x'' y'' EQ' EQ''] ??. red.
+    - intros ? INC x y [t t' u' u EQt HR EQu] ??. red.
       apply INC; auto.
       econstructor; eauto.
       apply leq_infx in H.
       now apply H.
-    - intros R IH x y [x' y' x'' y'' EQ' EQ''].
-      now subs.
+    - intros R IH x y [t t' u' u EQt HR EQu].
+      eapply Seq_ss'_gen_goal; [ exact EQt | symmetry; exact EQu | exact HR ].
   Qed.
 
-  #[global] Instance equ_clos_sst_goal {c: Chain (@ss' E F C D X Y L)} :
-    Proper (equ eq ==> equ eq ==> flip impl) `c.
+  #[global] Instance Seq_clos_sst_goal {c: Chain (@ss' E F B X L)} :
+    Proper (Seq ==> Seq ==> flip impl) `c.
   Proof.
     cbn; intros ? ? eq1 ? ? eq2 H.
-    apply equ_clos_sst'; econstructor; [eauto | | symmetry; eauto]; assumption.
+    apply Seq_clos_sst'; econstructor; [eauto | | symmetry; eauto]; assumption.
   Qed.
 
-  #[global] Instance equ_clos_sst'_ctx  {c: Chain (@ss' E F C D X Y L)} :
-    Proper (equ eq ==> equ eq ==> impl) `c.
+  #[global] Instance Seq_clos_sst'_ctx  {c: Chain (@ss' E F B X L)} :
+    Proper (Seq ==> Seq ==> impl) `c.
   Proof.
     cbn; intros ? ? eq1 ? ? eq2 H.
-    apply equ_clos_sst'; econstructor; [symmetry; eauto | | eauto]; assumption.
+    apply Seq_clos_sst'; econstructor; [symmetry; eauto | | eauto]; assumption.
   Qed.
 
-  #[global] Instance equ_clos_ssim'_goal : Proper (equ eq ==> equ eq ==> flip impl) (@ssim' E F C D X Y L).
+  #[global] Instance Seq_clos_ssim'_goal : Proper (Seq ==> Seq ==> flip impl) (@ssim' E F B X L).
   Proof.
     cbn; intros ? ? eq1 ? ? eq2 H.
-    apply equ_clos_sst'; econstructor; eauto; now symmetry.
+    apply Seq_clos_sst'; econstructor; eauto; now symmetry.
   Qed.
 
-  #[global] Instance equ_clos_ssim'_ctx : Proper (equ eq ==> equ eq ==> impl) (@ssim' E F C D X Y L).
+  #[global] Instance Seq_clos_ssim'_ctx : Proper (Seq ==> Seq ==> impl) (@ssim' E F B X L).
   Proof.
     cbn; intros ? ? eq1 ? ? eq2 H.
     now rewrite <- eq1, <- eq2.
   Qed.
 
-  Lemma ss'_gen_br : forall {Z} (c : C Z) (k : Z -> ctree E C X) (u : ctree F D Y)
-    (R Reps : rel _ _),
-    ss'_gen L R Reps (Br c k) u ->
-    forall x, exists u', epsilon u u' /\ Reps (k x) u'.
+  Lemma ss'_gen_epsilon_star {R : rel (@S E B X) (@S F B X)} :
+    forall (t t' : @S E B X) (u : @S F B X),
+    ss'_gen L R R t u ->
+    trans_alt ε t t' ->
+    exists u', (trans_alt ε)^* u u' /\ R t' u'.
   Proof.
-    intros. destruct H as (_ & H & _); eapply H; reflexivity.
+    intros * (_ & H); apply H.
   Qed.
 
-  Lemma ss'_gen_guard : forall (t : ctree E C X) (u : ctree F D Y)
-    (R Reps : rel _ _),
-    ss'_gen L R Reps (Guard t) u ->
-    exists u', epsilon u u' /\ Reps t u'.
+  Lemma trans_alt_estar_l {G : Type -> Type} :
+    forall (t t' : @S G B X) l,
+    trans_alt l t t' ->
+    ((trans_alt ε)^* ⋅ trans_alt l) t t'.
   Proof.
-    intros. destruct H as (_ & _ & H); eapply H; reflexivity.
+    intros. use_steps O. assumption.
   Qed.
 
 End ssim'_theory.
@@ -175,28 +210,28 @@ End ssim'_theory.
 Ltac fold_ssim' :=
   repeat
     match goal with
-    | h: context[gfp (@ss' ?E ?F ?C ?D ?X ?Y ?L)] |- _ =>
-        fold (@ssim' E F C D X Y L) in h
-    | |- context[gfp (@ss' ?E ?F ?C ?D ?X ?Y ?L)]      =>
-        fold (@ssim' E F C D X Y L)
+    | h: context[gfp (@ss' ?E ?F ?B ?X ?L)] |- _ =>
+        fold (@ssim' E F B X L) in h
+    | |- context[gfp (@ss' ?E ?F ?B ?X ?L)]      =>
+        fold (@ssim' E F B X L)
     end.
 
 Tactic Notation "__step_ssim'" :=
   match goal with
-  | |- context[@ssim' ?E ?F ?C ?D ?X ?Y ?LR] =>
+  | |- context[@ssim' ?E ?F ?B ?X ?L] =>
       unfold ssim';
       step;
-      fold (@ssim' E F C D X Y L)
+      fold (@ssim' E F B X L)
   end.
 
 Tactic Notation "step" := __step_ssim' || step.
 
 Ltac __step_in_ssim' H :=
   match type of H with
-  | context[@ssim' ?E ?F ?C ?D ?X ?Y ?LR] =>
+  | context[@ssim' ?E ?F ?B ?X ?L] =>
       unfold ssim' in H;
       step in H;
-      fold (@ssim' E F C D X Y L) in H
+      fold (@ssim' E F B X L) in H
   end.
 
 Tactic Notation "step" "in" ident(H) := __step_in_ssim' H || step in H.
@@ -209,29 +244,30 @@ Import CTreeNotations.
 Import EquNotations.
 Section ssim'_homogenous_theory.
   Context {E B: Type -> Type} {X: Type}
-          {L: relation (@label E)}.
+          {L: relation (@label E X)}.
 
-  Notation ss' := (@ss' E E B B X X).
-  Notation ssim' := (@ssim' E E B B X X).
+  Notation ss' := (@ss' E E B X).
+  Notation ssim' := (@ssim' E E B X).
+
 
   #[global] Instance Reflexive_ss' R Reps
-    `{Reflexive _ R} `{Reflexive _ Reps} `{Reflexive _ L}:
-    Reflexive (@ss'_gen E E B B X X L R Reps).
+    `{Reflexive _ R} `{Reflexive _ L} `{Reflexive _ Reps}:
+    Reflexive (@ss'_gen E E B X L R Reps).
   Proof.
-    split; [| split]; intros; eauto.
-    exists (k x0). subs. split; auto. now eapply epsilon_br.
+    split; intros.
+    exists l, t'. split; auto.  
+    use_steps O. assumption. 
     exists t'; split; eauto.
-    rewrite H2; now apply epsilon_guard.
+    use_steps (1 : nat). econstructor; eauto.  
   Qed.
 
   #[global] Instance refl_ss' {LR: Reflexive L} {C: Chain (ss' L)}: Reflexive `C.
   Proof.
     apply Reflexive_chain.
-    split; [| split]; cbn; intros; eauto.
-    - exists (k x0); split; auto.
-      rewrite H0; eapply epsilon_br, epsilon_id; reflexivity.
+    split; intros.
+    - do 2 eexists. split. use_steps O. apply H1. now split.  
     - exists t'; split; auto.
-      rewrite H0; eapply epsilon_guard, epsilon_id; reflexivity.
+      use_steps (1 : nat). econstructor; eauto. 
   Qed.
 
 End ssim'_homogenous_theory.
@@ -241,24 +277,23 @@ Parametric theory of [ss] with heterogenous [L]
 |*)
 Section ssim'_heterogenous_theory.
   Arguments label: clear implicits.
-  Context {E F C D: Type -> Type} {X Y: Type}
-          {L: rel (@label E) (@label F)}.
+  Context {E F B: Type -> Type} {X: Type}
+          {L: rel (@label E X) (@label F X)}.
 
-  Notation ss' := (@ss' E F C D X Y).
-  Notation ssim'  := (@ssim' E F C D X Y).
+  Notation ss' := (@ss' E F B X).
+  Notation ssim'  := (@ssim' E F B X).
 
 (*|
   stuck ctrees can be simulated by anything.
 |*)
   Lemma ss'_stuck R Reps :
-    forall (u : ctree F D Y),
-    ss'_gen (E := E) (C := C) (X := X) L R Reps Stuck u.
+    forall (u : @S F B X),
+    ss'_gen L R Reps (Stuck : ctree E B X) u.
   Proof.
-    split; [| split]; intros; inv_equ.
-    inv_trans.
+    split; intros; exfalso; eapply trans_stuck_inv; eassumption.
   Qed.
 
-  Lemma ssim'_stuck (t : ctree F D Y) : ssim' L Stuck t.
+  Lemma ssim'_stuck (t : @S F B X) : ssim' L (Stuck : ctree E B X) t.
   Proof.
     intros. step. apply ss'_stuck.
   Qed.
@@ -274,7 +309,7 @@ Ltac __play_ssim'_in H :=
 
 Ltac __eplay_ssim' :=
   match goal with
-  | h : @ssim' ?E ?F ?C ?D ?X ?Y ?L _ _ |- _ =>
+  | h : @ssim' ?E ?F ?B ?X ?L _ _ |- _ =>
       __play_ssim'_in h
   end.
 
@@ -285,41 +320,47 @@ Ltac __eplay_ssim' :=
 Section Proof_Rules.
 
   Arguments label: clear implicits.
-  Context {E F C D : Type -> Type}
-          {X Y : Type}
-          {L : rel (@label E) (@label F)}
-          {R Reps : rel (ctree E C X) (ctree F D Y)}
-          {HR : (Proper (equ eq ==> equ eq ==> impl) R)}
-          {HReps : (Proper (equ eq ==> equ eq ==> impl) Reps)}.
+  Context {E F B : Type -> Type}
+          {X : Type}
+          {L : rel (@label E X) (@label F X)}
+          {R Reps : rel (@S E B X) (@S F B X)}
+          {HR : (Proper (Seq ==> Seq ==> impl) R)}
+          {HReps : (Proper (Seq ==> Seq ==> impl) Reps)}.
 
   Lemma step_ss'_stuck :
-    ss'_gen L R Reps Stuck Stuck.
+    ss'_gen L R Reps (Stuck : ctree E B X) (Stuck : ctree F B X).
   Proof.
-    ssplit; intros; inv_equ.
-    exfalso; eapply productive_stuck; eauto.
+    split; intros; exfalso; eapply trans_stuck_inv; eassumption.
   Qed.
 
-  Lemma step_ss'_ret (x : X) (y : Y) :
+  Lemma step_ss'_ret (x : X) (y : X) :
     R Stuck Stuck ->
     L (val x) (val y) ->
-    ss'_gen L R Reps (Ret x : ctree E C X) (Ret y : ctree F D Y).
+    ss'_gen L R Reps (Ret x : ctree E B X) (Ret y : ctree F B X).
   Proof.
-    intros Rstuck Lval. split; [| split]; intros.
-    2,3: inv_equ.
-    inv_trans; subst.
-    do 3 eexists; intuition; etrans. now subs.
+    intros Rstuck Lval. split.
+    - intros t' l Hl TR. apply trans_ret_inv' in TR as (EQ & ->).
+      exists (val y), (Active Stuck). split; [| split].
+      + apply trans_alt_estar_l, trans_ret.
+      + rewrite EQ. apply Rstuck.
+      + assumption.
+    - intros t' TR. apply trans_ret_inv' in TR as (_ & abs). discriminate.
   Qed.
 
-  Lemma step_ss'_ret_l (x : X) (y : Y) (u u' : ctree F D Y) :
+  Lemma step_ss'_ret_l (x : X) (y : X) (u u' : @S F B X) :
     R Stuck Stuck ->
     L (val x) (val y) ->
-    trans (val y) u u' ->
-    ss'_gen L R Reps (Ret x : ctree E C X) u.
+    trans_alt (val y) u u' ->
+    ss'_gen L R Reps (Ret x : ctree E B X) u.
   Proof.
-    intros. cbn. intros.
-    apply trans_val_inv in H1 as ?. subs.
-    split; [| split]; intros; inv_equ.
-    inv_trans. subst. rewrite <- EQ in H. etrans.
+    intros Rstuck Lval TR. split.
+    - intros t' l Hl TRl. apply trans_ret_inv' in TRl as (EQ & ->).
+      pose proof (trans_val_inv' TR) as EQ'.
+      exists (val y), u'. split; [| split].
+      + apply trans_alt_estar_l, TR.
+      + rewrite EQ, EQ'. apply Rstuck.
+      + assumption.
+    - intros t' TRl. apply trans_ret_inv' in TRl as (_ & abs). discriminate.
   Qed.
 
 (*|
@@ -328,82 +369,153 @@ Section Proof_Rules.
  the itree-style rule.
 |*)
   Lemma step_ss'_vis {Z Z'} (e : E Z) (f: F Z')
-        (k : Z -> ctree E C X) (k' : Z' -> ctree F D Y) :
-    (forall x, exists y, R (k x) (k' y) /\ L (obs e x) (obs f y)) ->
+        (k : Z -> ctree E B X) (k' : Z' -> ctree F B X) :
+    R (Passive e k) (Passive f k') ->
+    L (ask e) (ask f) ->
     ss'_gen L R Reps (Vis e k) (Vis f k').
   Proof.
-    intros. split; [| split]; intros; inv_equ.
-    cbn; inv_trans; subst;
-      destruct (H x) as (x' & RR & LL);
-      cbn; do 3 eexists; intuition.
-    - rewrite EQ; eauto.
-    - assumption.
+    intros HRpas Lask. split.
+    - intros t' l Hl TR. apply trans_vis_inv' in TR as (EQ & ->).
+      exists (ask f), (Passive f k'). split; [| split].
+      + apply trans_alt_estar_l, trans_ask.
+      + rewrite EQ. apply HRpas.
+      + assumption.
+    - intros t' TR. apply trans_vis_inv' in TR as (_ & abs). discriminate.
   Qed.
 
   Lemma step_ss'_vis_id {Z} (e : E Z) (f: F Z)
-        (k : Z -> ctree E C X) (k' : Z -> ctree F D Y) :
-    (forall x, R (k x) (k' x) /\ L (obs e x) (obs f x)) ->
+        (k : Z -> ctree E B X) (k' : Z -> ctree F B X) :
+    R (Passive e k) (Passive f k') ->
+    L (ask e) (ask f) ->
     ss'_gen L R Reps (Vis e k) (Vis f k').
   Proof.
-    intros. apply step_ss'_vis.
-    eauto.
+    intros; apply step_ss'_vis; auto.
   Qed.
 
   Lemma step_ss'_vis_l {Z} :
-    forall (e : E Z) (k : Z -> ctree E C X) (u : ctree F D Y),
-    (forall x, exists l' u', trans l' u u' /\ R (k x) u' /\ L (obs e x) l') ->
+    forall (e : E Z) (k : Z -> ctree E B X) (u : @S F B X),
+    (exists l' u', ((trans_alt ε)^* ⋅ trans_alt l') u u' /\ R (Passive e k) u' /\ L (ask e) l') ->
     ss'_gen L R Reps (Vis e k) u.
   Proof.
-    intros. split; [| split]; intros; inv_equ.
-    inv_trans. subst. destruct (H x) as (? & ? & ? & ? & ?).
-    eexists _, _. rewrite <- EQ in H2. etrans.
+    intros e k u (l' & u' & STEP & HRu & Lask). split.
+    - intros t' l Hl TR. apply trans_vis_inv' in TR as (EQ & ->).
+      exists l', u'. split; [| split].
+      + assumption.
+      + rewrite EQ. assumption.
+      + assumption.
+    - intros t' TR. apply trans_vis_inv' in TR as (_ & abs). discriminate.
   Qed.
 
 (*|
     With this definition [ss'] of simulation, delayed nodes allow to perform a coinductive step.
 |*)
-  Lemma step_ss'_br_l {Z} (c : C Z)
-        (k : Z -> ctree E C X) (t': ctree F D Y):
-    (forall x, Reps (k x) t') ->
-    ss'_gen L R Reps (Br c k) t'.
+  Lemma trans_alt_br_inv {G : Type -> Type} {Z} (c : B Z) (k : Z -> ctree G B X) l u :
+    trans_alt l (Br c k) u -> l = ε /\ exists x, u ⩸ (Active (k x)).
   Proof.
-    ssplit; intros.
-    now apply productive_br in H0.
-    inv_equ. exists t'; split; eauto; rewrite <- EQ; auto.
-    inv_equ.
+    intros TR; unfold trans_alt in TR; cbn in TR.
+    dependent induction TR; inv_equ.
+    split; auto.
+    eexists; constructor.
+    rewrite H0; first [ now apply EQ | now symmetry; apply EQ
+                      | now rewrite EQ | now rewrite <- EQ ].
   Qed.
 
-  Lemma step_ss'_br_r {Z} (c : D Z) x
-        (k : Z -> ctree F D Y) (t: ctree E C X):
+  Lemma trans_alt_guard_inv {G : Type -> Type} (t : ctree G B X) l u :
+    trans_alt l (Guard t) u -> l = ε /\ u ⩸ (Active t).
+  Proof.
+    intros TR; unfold trans_alt in TR; cbn in TR.
+    dependent induction TR; inv_equ.
+    split; auto.
+    constructor.
+    first [ now rewrite H0, <- H | now rewrite H0, H
+          | now (rewrite H0; symmetry) ].
+  Qed.
+
+  Lemma step_ss'_br_l {Z} (c : B Z)
+        (k : Z -> ctree E B X) (u : @S F B X):
+    (forall x, Reps (Active (k x)) u) ->
+    ss'_gen L R Reps (Br c k) u.
+  Proof.
+    intros HReps'. split.
+    - intros t' l Hl TR. apply trans_alt_br_inv in TR as (-> & _). easy.
+    - intros t' TR. apply trans_alt_br_inv in TR as (_ & x & EQ).
+      exists u; split.
+      + apply (str_refl (trans_alt ε)); cbn; reflexivity.
+      + rewrite EQ. apply HReps'.
+  Qed.
+
+  Lemma estar_trans {G : Type -> Type} (a b c : @S G B X) :
+    (trans_alt ε)^* a b -> (trans_alt ε)^* b c -> (trans_alt ε)^* a c.
+  Proof.
+    intros S1 S2.
+    assert (H : (@trans_alt G B X ε)^* ⋅ (trans_alt ε)^* ≦ (trans_alt ε)^*) by ka.
+    apply H; eexists; eassumption.
+  Qed.
+
+  Lemma estar_cons0 {G : Type -> Type} (a b c : @S G B X) :
+    trans_alt ε a b -> (trans_alt ε)^* b c -> (trans_alt ε)^* a c.
+  Proof.
+    intros S1 S2.
+    assert (H : @trans_alt G B X ε ⋅ (trans_alt ε)^* ≦ (trans_alt ε)^*) by ka.
+    apply H; eexists; eassumption.
+  Qed.
+
+  Lemma estar_single {G : Type -> Type} (a b : @S G B X) :
+    trans_alt ε a b -> (trans_alt ε)^* a b.
+  Proof.
+    intro S; eapply estar_cons0; [ exact S | apply trans_star_self ].
+  Qed.
+
+  Lemma estar_cons {G : Type -> Type} (a b c : @S G B X) l :
+    trans_alt ε a b -> ((trans_alt ε)^* ⋅ trans_alt l) b c ->
+    ((trans_alt ε)^* ⋅ trans_alt l) a c.
+  Proof.
+    intros S1 S2.
+    assert (H : @trans_alt G B X ε ⋅ ((trans_alt ε)^* ⋅ trans_alt l)
+                ≦ (trans_alt ε)^* ⋅ trans_alt l) by ka.
+    apply H; eexists; eassumption.
+  Qed.
+
+  Lemma estar_app {G : Type -> Type} (a b c : @S G B X) l :
+    (trans_alt ε)^* a b -> ((trans_alt ε)^* ⋅ trans_alt l) b c ->
+    ((trans_alt ε)^* ⋅ trans_alt l) a c.
+  Proof.
+    intros S1 S2.
+    assert (H : (@trans_alt G B X ε)^* ⋅ ((trans_alt ε)^* ⋅ trans_alt l)
+                ≦ (trans_alt ε)^* ⋅ trans_alt l) by ka.
+    apply H; eexists; eassumption.
+  Qed.
+
+  Lemma step_ss'_br_r {Z} (c : B Z) x
+        (k : Z -> ctree F B X) (t: @S E B X):
     ss'_gen L R Reps t (k x) ->
     ss'_gen L R Reps t (Br c k).
   Proof.
-    intros (HA & HB & HC); ssplit; intros.
-    - apply HA in H0 as (? & ? & ? & ? & ?).
-      exists x0, x1; etrans. auto.
-    - eapply HB in H as (? & ? & ?). eapply epsilon_br in H. etrans.
-    - eapply HC in H as (? & ? & ?).
-      eexists; split; [| eauto].
-      eapply epsilon_br, H.
+    intros (HA & HB); split.
+    - intros t' l Hl TR. apply HA in TR as (l' & u' & STEP & HRtu & HL); auto.
+      exists l', u'; split; [| split; assumption].
+      eapply estar_cons; [ apply trans_br | exact STEP ].
+    - intros t' TR. apply HB in TR as (u' & STEP & HRep).
+      exists u'; split; [| assumption].
+      eapply estar_cons0; [ apply trans_br | exact STEP ].
   Qed.
 
-  Lemma step_ss'_br {Z Z'} (a: C Z) (b: D Z')
-    (k : Z -> ctree E C X) (k' : Z' -> ctree F D Y) :
+  Lemma step_ss'_br {Z Z'} (a: B Z) (b: B Z')
+    (k : Z -> ctree E B X) (k' : Z' -> ctree F B X) :
     (forall x, exists y, Reps (k x) (k' y)) ->
     ss'_gen L R Reps (Br a k) (Br b k').
   Proof.
-    ssplit; intros. { now apply productive_br in H0. }
-    2: inv_equ.
-    inv_equ.
-    setoid_rewrite EQ in H. destruct (H x).
-    eexists. split; [| eassumption].
-    econstructor 2.
-    econstructor.
-    reflexivity.
+    intros HRep; split.
+    - intros t' l Hl TR. apply trans_alt_br_inv in TR as (-> & _); easy.
+    - intros t' TR. apply trans_alt_br_inv in TR as (_ & x & EQ).
+      destruct (HRep x) as (y & HR').
+      exists (Active (k' y)); split.
+      + apply estar_single, trans_br.
+      + rewrite EQ. apply HR'.
   Qed.
 
-  Lemma step_ss'_br_id {Z} (c: C Z) (d: D Z)
-        (k : Z -> ctree E C X) (k' : Z -> ctree F D Y) :
+  Lemma step_ss'_br_id {Z} (c: B Z) (d: B Z)
+        (k : Z -> ctree E B X) (k' : Z -> ctree F B X) :
     (forall x, Reps (k x) (k' x)) ->
     ss'_gen L R Reps (Br c k) (Br d k').
   Proof.
@@ -411,103 +523,105 @@ Section Proof_Rules.
   Qed.
 
   Lemma step_ss'_guard_l
-        (t: ctree E C X) (t': ctree F D Y) :
-    Reps t t' ->
-    ss'_gen L R Reps (Guard t) t'.
+        (t: ctree E B X) (u: @S F B X) :
+    Reps t u ->
+    ss'_gen L R Reps (Guard t) u.
   Proof.
-    ssplit; intros.
-    now apply productive_guard in H0.
-    inv_equ.
-    inv_equ.
-    eexists t'; split.
-    reflexivity.
-    rewrite <- H0; auto.
+    intros HRep; split.
+    - intros t' l Hl TR. apply trans_alt_guard_inv in TR as (-> & _); easy.
+    - intros t' TR. apply trans_alt_guard_inv in TR as (_ & EQ).
+      exists u; split; [ apply trans_star_self | rewrite EQ; apply HRep ].
   Qed.
 
   Lemma step_ss'_guard_r
-    (t: ctree E C X) (t': ctree F D Y) :
+    (t: @S E B X) (t': ctree F B X) :
     ss'_gen L R Reps t t' ->
     ss'_gen L R Reps t (Guard t').
   Proof.
-    intros (HA & HB & HC); ssplit; intros.
-    - apply HA in H0 as (? & ? & ? & ? & ?).
-      do 2 eexists; etrans.
-      auto.
-    - eapply HB in H as (? & ? & ?).
-      eexists; split; [| eauto].
-      eapply epsilon_guard, H.
-    - eapply HC in H as (? & ? & ?).
-      eexists; split; [| eauto].
-      eapply epsilon_guard, H.
+    intros (HA & HB); split.
+    - intros s l Hl TR. apply HA in TR as (l' & u' & STEP & HRtu & HL); auto.
+      exists l', u'; split; [| split; assumption].
+      eapply estar_cons; [ apply trans_guard | exact STEP ].
+    - intros s TR. apply HB in TR as (u' & STEP & HRep).
+      exists u'; split; [| assumption].
+      eapply estar_cons0; [ apply trans_guard | exact STEP ].
   Qed.
 
   Lemma step_ss'_guard
-        (t: ctree E C X) (t': ctree F D Y) :
+        (t: ctree E B X) (t': ctree F B X) :
     Reps t t' ->
     ss'_gen L R Reps (Guard t) (Guard t').
   Proof.
-    ssplit; intros. { now apply productive_guard in H0. }
-    inv_equ.
-    inv_equ.
-    setoid_rewrite H0 in H.
-    eexists. split; [| eassumption].
-    now econstructor 3.
+    intros HRep; split.
+    - intros s l Hl TR. apply trans_alt_guard_inv in TR as (-> & _); easy.
+    - intros s TR. apply trans_alt_guard_inv in TR as (_ & EQ).
+      exists (Active t'); split.
+      + apply estar_single, trans_guard.
+      + rewrite EQ. apply HRep.
   Qed.
 
   Lemma step_ss'_epsilon_r :
-    forall (t : ctree E C X) (u u' : ctree F D Y),
-      ss'_gen L R Reps t u' -> epsilon u u' -> ss'_gen L R Reps t u.
+    forall (t : @S E B X) (u u' : @S F B X),
+      ss'_gen L R Reps t u' -> (trans_alt ε)^* u u' -> ss'_gen L R Reps t u.
   Proof.
-    intros. red in H0. rewrite (ctree_eta u). rewrite (ctree_eta u') in H.
-    genobs u ou. genobs u' ou'. clear u Heqou u' Heqou'.
-    revert t H. induction H0; intros.
-    - now subs.
-    - eapply step_ss'_br_r, IHepsilon_; eauto.
-    - eapply step_ss'_guard_r, IHepsilon_; eauto.
+    intros t u u' (HA & HB) STAR; split.
+    - intros s l Hl TR. apply HA in TR as (l' & u'' & STEP & HRtu & HL); auto.
+      exists l', u''; split; [| split; assumption].
+      eapply estar_app; eassumption.
+    - intros s TR. apply HB in TR as (u'' & STEP & HRep).
+      exists u''; split; [| assumption].
+      eapply estar_trans; eassumption.
   Qed.
 
   Lemma ss'_gen_epsilon_l :
-    forall (t t' : ctree E C X) (u : ctree F D Y),
+    forall (t t' : @S E B X) (u : @S F B X),
     Reps <= ss'_gen L R Reps ->
     ss'_gen L R Reps t u ->
-    epsilon t t' ->
+    (trans_alt ε)^* t t' ->
     ss'_gen L R Reps t' u.
   Proof.
-    intros. red in H1. rewrite (ctree_eta t'). rewrite (ctree_eta t) in H0.
-    genobs t ot. genobs t' ot'. clear t Heqot t' Heqot'.
-    revert u H0. induction H1; intros.
-    - now subs.
-    - apply IHepsilon_. rewrite <- ctree_eta.
-      eapply ss'_gen_br in H0 as (? & ? & ?).
-      apply H in H2. eapply step_ss'_epsilon_r in H2; eauto.
-    - apply IHepsilon_. rewrite <- ctree_eta.
-      eapply ss'_gen_guard in H0 as (? & ? & ?).
-      apply H in H2. eapply step_ss'_epsilon_r in H2; eauto.
-   Qed.
-
+    intros t t' u HRle HSS STAR.
+    destruct STAR as [n STAR]. revert t t' u HRle HSS STAR.
+    induction n; intros t t' u HRle HSS STAR.
+    - cbn in STAR. now rewrite STAR in HSS.
+    - destruct STAR as [m STEP REST].
+      destruct HSS as (HA & HB).
+      apply HB in STEP as (u' & STARu & HRep).
+      apply HRle in HRep.
+      eapply step_ss'_epsilon_r in HRep; [| exact STARu].
+      eapply IHn; [ exact HRle | exact HRep | exact REST ].
+  Qed.
 
   (*|
     Same goes for visible τ nodes.
     |*)
   Lemma step_ss'_step
-        (t : ctree E C X) (t': ctree F D Y) :
+        (t : ctree E B X) (t': ctree F B X) :
     L τ τ ->
     R t t' ->
     ss'_gen L R Reps (Step t) (Step t').
   Proof.
-    split; [| split]; intros; inv_equ.
-    inv_trans; subst.
-    cbn; do 3 eexists; intuition; subs; eauto.
+    intros Ltau HRtt; split.
+    - intros s l Hl TR. apply trans_step_inv' in TR as (EQ & ->).
+      exists τ, (Active t'). split; [| split].
+      + apply trans_alt_estar_l, trans_step.
+      + rewrite EQ. apply HRtt.
+      + assumption.
+    - intros s TR. apply trans_step_inv' in TR as (_ & abs). discriminate.
   Qed.
 
   Lemma step_ss'_step_l :
-    forall (t : ctree E C X) (u : ctree F D Y),
-    (exists l' u', trans l' u u' /\ R t u' /\ L τ l') ->
+    forall (t : ctree E B X) (u : @S F B X),
+    (exists l' u', ((trans_alt ε)^* ⋅ trans_alt l') u u' /\ R t u' /\ L τ l') ->
     ss'_gen L R Reps (Step t) u.
   Proof.
-    intros. ssplit; intros; inv_equ.
-    inv_trans. subst. destruct H as (? & ? & ? & ? & ?).
-    eexists _, _. rewrite <- EQ in H1. etrans.
+    intros t u (l' & u' & STEP & HRtu & Ltau). split.
+    - intros s l Hl TR. apply trans_step_inv' in TR as (EQ & ->).
+      exists l', u'. split; [| split].
+      + assumption.
+      + rewrite EQ. assumption.
+      + assumption.
+    - intros s TR. apply trans_step_inv' in TR as (_ & abs). discriminate.
   Qed.
 
 (*|
@@ -521,34 +635,34 @@ End Proof_Rules.
 
 (* Specialized proof rules *)
 
-Lemma ssim'_stuck' {E F C D X Y}
+Lemma ssim'_stuck' {E F B X}
   (L : rel _ _) :
-  ssim' L (Stuck : ctree E C X) (Stuck : ctree F D Y).
+  ssim' L (Stuck : ctree E B X) (Stuck : ctree F B X).
 Proof.
   step. apply step_ss'_stuck.
 Qed.
 
-Lemma step_ssbt'_ret {E F C D X Y}
-  (x : X) (y : Y) (L : rel _ _)
-  {R : Chain (@ss' E F C D X Y L)} :
+Lemma step_ssbt'_ret {E F B X}
+  (x : X) (y : X) (L : rel _ _)
+  {R : Chain (@ss' E F B X L)} :
   L (val x) (val y) ->
-  ss' L `R (Ret x : ctree E C X) (Ret y : ctree F D Y).
+  ss' L `R (Ret x : ctree E B X) (Ret y : ctree F B X).
 Proof.
   intros.
   unshelve eapply step_ss'_ret; eauto.
   apply (b_chain R). apply ss'_stuck.
 Qed.
 
-Lemma ssim'_ret {E F C D X Y}
-  (x : X) (y : Y) (L : rel _ _) :
+Lemma ssim'_ret {E F B X}
+  (x : X) (y : X) (L : rel _ _) :
   L (val x) (val y) ->
-  ssim' L (Ret x : ctree E C X) (Ret y : ctree F D Y).
+  ssim' L (Ret x : ctree E B X) (Ret y : ctree F B X).
 Proof.
   now intros; step; apply step_ssbt'_ret.
 Qed.
 
-Lemma ssim'_step {E F C D X Y}
-  (t : ctree E C X) (u : ctree F D Y) (L : rel _ _) :
+Lemma ssim'_step {E F B X}
+  (t : ctree E B X) (u : ctree F B X) (L : rel _ _) :
   L τ τ  ->
   ssim' L t u ->
   ssim' L (Step t) (Step u).
@@ -556,36 +670,36 @@ Proof.
   now intros; step; apply step_ss'_step.
 Qed.
 
-Lemma ssim'_guard {E F C D X Y}
-  (t : ctree E C X) (u : ctree F D Y) (L : rel _ _) :
+Lemma ssim'_guard {E F B X}
+  (t : ctree E B X) (u : ctree F B X) (L : rel _ _) :
   ssim' L t u ->
   ssim' L (Guard t) (Guard u).
 Proof.
   now intros; step; apply step_ss'_guard.
 Qed.
 
-Lemma ssim'_br {E F C D X Y Z Z'} {L}
-  (c: C Z) (d: D Z')
-  (k : Z -> ctree E C X) (k' : Z' -> ctree F D Y) :
+Lemma ssim'_br {E F B X Z Z'} {L}
+  (c: B Z) (d: B Z')
+  (k : Z -> ctree E B X) (k' : Z' -> ctree F B X) :
   (forall x, exists y, ssim' L (k x) (k' y)) ->
   ssim' L (Br c k) (Br d k').
 Proof.
   now intros; step; apply step_ss'_br.
 Qed.
 
-Lemma ssim'_br_id {E F C D X Y Z} {L}
-  (c: C Z) (d: D Z)
-  (k : Z -> ctree E C X) (k' : Z -> ctree F D Y) :
+Lemma ssim'_br_id {E F B X Z} {L}
+  (c: B Z) (d: B Z)
+  (k : Z -> ctree E B X) (k' : Z -> ctree F B X) :
   (forall x, ssim' L (k x) (k' x)) ->
   ssim' L (Br c k) (Br d k').
 Proof.
   now intros; step; apply step_ss'_br_id.
 Qed.
 
-Lemma step_ssbt'_brS {E F C D X Y Z Z'} {L}
-  {R : Chain (@ss' E F C D X Y L)}
-  (c: C Z) (d: D Z')
-  (k : Z -> ctree E C X) (k' : Z' -> ctree F D Y) :
+Lemma step_ssbt'_brS {E F B X Z Z'} {L}
+  {R : Chain (@ss' E F B X L)}
+  (c: B Z) (d: B Z')
+  (k : Z -> ctree E B X) (k' : Z' -> ctree F B X) :
   L τ τ  ->
   (forall x, exists y, `R (k x) (k' y)) ->
   ss' L `R (BrS c k) (BrS d k').
@@ -596,9 +710,9 @@ Proof.
   apply (b_chain R), step_ss'_step; auto.
 Qed.
 
-Lemma ssim'_brS {E F C D X Y Z Z'} {L}
-  (c: C Z) (d: D Z')
-  (k : Z -> ctree E C X) (k' : Z' -> ctree F D Y) :
+Lemma ssim'_brS {E F B X Z Z'} {L}
+  (c: B Z) (d: B Z')
+  (k : Z -> ctree E B X) (k' : Z' -> ctree F B X) :
   L τ τ  ->
   (forall x, exists y, ssim' L (k x) (k' y)) ->
   ssim' L (BrS c k) (BrS d k').
@@ -606,10 +720,10 @@ Proof.
   now intros; step; apply step_ssbt'_brS.
 Qed.
 
-Lemma step_ssbt'_brS_id {E F C D X Y Z} {L}
-  {R : Chain (@ss' E F C D X Y L)}
-  (c: C Z) (d: D Z)
-  (k : Z -> ctree E C X) (k' : Z -> ctree F D Y) :
+Lemma step_ssbt'_brS_id {E F B X Z} {L}
+  {R : Chain (@ss' E F B X L)}
+  (c: B Z) (d: B Z)
+  (k : Z -> ctree E B X) (k' : Z -> ctree F B X) :
   L τ τ  ->
   (forall x, ` R (k x) (k' x)) ->
   ss' L `R (BrS c k) (BrS d k').
@@ -619,9 +733,9 @@ Proof.
   intros; apply (b_chain R), step_ss'_step; auto.
 Qed.
 
-Lemma ssim'_brS_id {E F C D X Y Z} {L}
-  (c: C Z) (d: D Z)
-  (k : Z -> ctree E C X) (k' : Z -> ctree F D Y) :
+Lemma ssim'_brS_id {E F B X Z} {L}
+  (c: B Z) (d: B Z)
+  (k : Z -> ctree E B X) (k' : Z -> ctree F B X) :
   L τ τ  ->
   (forall x, ssim' L (k x) (k' x)) ->
   ssim' L (BrS c k) (BrS d k').
@@ -630,39 +744,41 @@ Proof.
 Qed.
 
 Lemma ssim'_vis
-  {E F C D X Y Z Z'} {L}
+  {E F B X Z Z'} {L}
   (e: E Z) (f: F Z')
-  (k : Z -> ctree E C X) (k' : Z' -> ctree F D Y) :
-  (forall x, exists y, ssim' L (k x) (k' y) /\ L (obs e x) (obs f y)) ->
+  (k : Z -> ctree E B X) (k' : Z' -> ctree F B X) :
+  ssim' L (Passive e k) (Passive f k') ->
+  L (ask e) (ask f) ->
   ssim' L (Vis e k) (Vis f k').
 Proof.
-  now intros; step; apply step_ss'_vis.
+  intros Hpas Hask; step; apply step_ss'_vis; [exact Hpas | exact Hask].
 Qed.
 
 Lemma ssim'_vis_id
-  {E F C D X Y Z} {L}
+  {E F B X Z} {L}
   (e: E Z) (f: F Z)
-  (k : Z -> ctree E C X) (k' : Z -> ctree F D Y) :
-  (forall x, ssim' L (k x) (k' x) /\ L (obs e x) (obs f x)) ->
+  (k : Z -> ctree E B X) (k' : Z -> ctree F B X) :
+  ssim' L (Passive e k) (Passive f k') ->
+  L (ask e) (ask f) ->
   ssim' L (Vis e k) (Vis f k').
 Proof.
-  now intros; step; apply step_ss'_vis_id.
+  intros Hpas Hask; step; apply step_ss'_vis_id; [exact Hpas | exact Hask].
 Qed.
 
 Lemma ssim'_vis_l
-  {E F C D X Y Z} {L}
+  {E F B X Z} {L}
   (e: E Z)
-  (k : Z -> ctree E C X) (u : ctree F D Y) :
-  (forall x, exists l' u', trans l' u u' /\ ssim' L (k x) u' /\ L (obs e x) l') ->
+  (k : Z -> ctree E B X) (u : @S F B X) :
+  (exists l' u', ((trans_alt ε)^* ⋅ trans_alt l') u u' /\ ssim' L (Passive e k) u' /\ L (ask e) l') ->
   ssim' L (Vis e k) u.
 Proof.
-  now intros; step; apply step_ss'_vis_l.
+  intros H; step; apply step_ss'_vis_l; exact H.
 Qed.
 
-Lemma ssim'_epsilon_l {E F C D X Y} {L} :
-  forall (t t' : ctree E C X) (u : ctree F D Y),
+Lemma ssim'_epsilon_l {E F B X} {L} :
+  forall (t t' : @S E B X) (u : @S F B X),
   ssim' L t u ->
-  epsilon t t' ->
+  (trans_alt ε)^* t t' ->
   ssim' L t' u.
 Proof.
   intros. step. eapply ss'_gen_epsilon_l.
@@ -673,36 +789,37 @@ Qed.
 
 Section Inversion_Rules.
 
-  Context {E F C D : Type -> Type}
-          {X Y : Type}
-          {L : rel (@label E) (@label F)}
-          {R Reps : rel (ctree E C X) (ctree F D Y)}.
+  Context {E F B : Type -> Type}
+          {X : Type}
+          {L : rel (@label E X) (@label F X)}
+          {R Reps : rel (@S E B X) (@S F B X)}.
 
   Lemma ss'_vis_l_inv {Z} :
-    forall (e : E Z) (k : Z -> ctree E C X) (u : ctree F D Y) x,
+    forall (e : E Z) (k : Z -> ctree E B X) (u : @S F B X),
     ss'_gen L R Reps (Vis e k) u ->
-    exists l' u', trans l' u u' /\ R (k x) u' /\ L (obs e x) l'.
+    exists l' u', ((trans_alt ε)^* ⋅ trans_alt l') u u' /\ R (Passive e k) u' /\ L (ask e) l'.
   Proof.
-    intros. apply H; etrans.
+    intros e k u (HA & _).
+    apply (HA (Passive e k) (ask e)); [ discriminate | apply trans_ask ].
   Qed.
 
   Lemma ss'_step_l_inv :
-    forall (t : ctree E C X) (u : ctree F D Y),
+    forall (t : ctree E B X) (u : @S F B X),
     ss'_gen L R Reps (Step t) u ->
-    exists l' u', trans l' u u' /\ R t u' /\ L τ l'.
+    exists l' u', ((trans_alt ε)^* ⋅ trans_alt l') u u' /\ R t u' /\ L τ l'.
   Proof.
-    intros * (HA & HB & HC).
-    apply HA; etrans.
+    intros t u (HA & _).
+    apply (HA (Active t) τ); [ discriminate | apply trans_step ].
   Qed.
 
 End Inversion_Rules.
 
-Definition epsilon_ctx {E C X} (R : ctree E C X -> Prop)
-  (t : ctree E C X) :=
+Definition epsilon_ctx {E B X} (R : ctree E B X -> Prop)
+  (t : ctree E B X) :=
   exists t', epsilon t t' /\ R t'.
 
-Definition epsilon_det_ctx {E C X} (R : ctree E C X -> Prop)
-  (t : ctree E C X) :=
+Definition epsilon_det_ctx {E B X} (R : ctree E B X -> Prop)
+  (t : ctree E B X) :=
   exists t', epsilon_det t t' /\ R t'.
 
 Section upto.
@@ -712,7 +829,7 @@ Section upto.
 
   (* Up-to epsilon *)
 
-  Program Definition epsilon_ctx_r : mon (rel (ctree E C X) (ctree F D Y))
+  Program Definition epsilon_ctx_r : mon (rel (ctree E B X) (ctree F B X))
     := {| body R t u := epsilon_ctx (fun u => R t u) u |}.
   Next Obligation.
     destruct H0 as (? & ? & ?). red. eauto.
@@ -785,7 +902,7 @@ Section upto.
 
 End upto.
 
-Arguments ss_sst' {E F C D X Y} L.
+Arguments ss_sst' {E F B X} L.
 
 (*|
 Up-to [bind] context simulations
@@ -809,7 +926,7 @@ Section bind.
   Lemma bind_chain_gen L0
     (ISVR : is_update_val_rel L R0 L0)
     {R : Chain (@ss' E F C D X' Y' L)} :
-    forall (t : ctree E C X) (t' : ctree F D Y) (k : X -> ctree E C X') (k' : Y -> ctree F D Y'),
+    forall (t : ctree E B X) (t' : ctree F B X) (k : X -> ctree E B X') (k' : Y -> ctree F B X'),
       ssim L0 t t' ->
       (forall x x', R0 x x' -> elem R (k x) (k' x')) ->
       ` R (bind t k) (bind t' k').
@@ -897,8 +1014,8 @@ Expliciting the reasoning rule provided by the up-to principles.
 Lemma ss'_clo_bind_gen {E F C D: Type -> Type} {X Y X' Y': Type}  {L : rel (@label E) (@label F)}
       (R0 : rel X Y) L0
       (HL0 : is_update_val_rel L R0 L0)
-      (t1 : ctree E C X) (t2: ctree F D Y)
-      (k1 : X -> ctree E C X') (k2 : Y -> ctree F D Y'):
+      (t1 : ctree E B X) (t2: ctree F B X)
+      (k1 : X -> ctree E B X') (k2 : Y -> ctree F B X'):
   ssim L0 t1 t2 ->
   (forall x y, R0 x y -> ssim' L (k1 x) (k2 y)) ->
   ssim' L (t1 >>= k1) (t2 >>= k2).
@@ -910,7 +1027,7 @@ Qed.
 Lemma ss'_clo_bind {E F C D: Type -> Type} {X Y X' Y': Type} {L : rel (@label E) (@label F)}
   (R0 : rel X Y)
   {R : Chain (@ss' E F C D X' Y' L)} :
-  forall (t : ctree E C X) (t' : ctree F D Y) (k : X -> ctree E C X') (k' : Y -> ctree F D Y'),
+  forall (t : ctree E B X) (t' : ctree F B X) (k : X -> ctree E B X') (k' : Y -> ctree F B X'),
     t (≲update_val_rel L R0) t' ->
     (forall x x', R0 x x' -> elem R (k x) (k' x')) ->
     ` R (bind t k) (bind t' k').
@@ -921,8 +1038,8 @@ Qed.
 
 Lemma ssim'_clo_bind {E F C D: Type -> Type} {X Y X' Y': Type} {L : rel (@label E) (@label F)}
       (R0 : rel X Y)
-      (t1 : ctree E C X) (t2: ctree F D Y)
-      (k1 : X -> ctree E C X') (k2 : Y -> ctree F D Y'):
+      (t1 : ctree E B X) (t2: ctree F B X)
+      (k1 : X -> ctree E B X') (k2 : Y -> ctree F B X'):
   t1 (≲update_val_rel L R0) t2 ->
   (forall x y, R0 x y -> ssim' L (k1 x) (k2 y)) ->
   ssim' L (t1 >>= k1) (t2 >>= k2).
@@ -932,7 +1049,7 @@ Qed.
 
 Lemma ss'_clo_bind_eq {E C D: Type -> Type} {X X': Type}
   {R : Chain (@ss' E E C D X' X' eq)} :
-  forall (t : ctree E C X) (t' : ctree E D X) (k : X -> ctree E C X') (k' : X -> ctree E D X'),
+  forall (t : ctree E B X) (t' : ctree E D X) (k : X -> ctree E B X') (k' : X -> ctree E D X'),
     t ≲ t' ->
     (forall x, elem R (k x) (k' x)) ->
     ` R (bind t k) (bind t' k').
@@ -944,8 +1061,8 @@ Proof.
 Qed.
 
 Lemma ssim'_clo_bind_eq {E C D: Type -> Type} {X X': Type}
-      (t1 : ctree E C X) (t2: ctree E D X)
-      (k1 : X -> ctree E C X') (k2 : X -> ctree E D X'):
+      (t1 : ctree E B X) (t2: ctree E D X)
+      (k1 : X -> ctree E B X') (k2 : X -> ctree E D X'):
   t1 ≲ t2 ->
   (forall x, ssim' eq (k1 x) (k2 x)) ->
   ssim' eq (t1 >>= k1) (t2 >>= k2).
@@ -953,8 +1070,8 @@ Proof.
   apply ss'_clo_bind_eq.
 Qed.
 
-Lemma ss_ss'_chain {E F C D X Y L} {R : Chain (ss' L)} :
-  forall (t : ctree E C X) (u : ctree F D Y),
+Lemma ss_ss'_chain {E F B X L} {R : Chain (ss' L)} :
+  forall (t : ctree E B X) (u : ctree F B X),
   ss L `R t u ->
   ss' L `R t u.
 Proof.
@@ -968,8 +1085,8 @@ Proof.
 Qed.
 
 (* This alternative notion of simulation is equivalent to [ssim] *)
-Theorem ssim_ssim' {E F C D X Y} :
-  forall L (t : ctree E C X) (t' : ctree F D Y), ssim L t t' <-> ssim' L t t'.
+Theorem ssim_ssim' {E F B X} :
+  forall L (t : ctree E B X) (t' : ctree F B X), ssim L t t' <-> ssim' L t t'.
 Proof.
   split; intros.
   - red. revert t t' H. coinduction R CH. intros.
