theories/Eq/Trace.v
@@ -14,15 +14,16 @@ From CTree Require Import
 Base coinductive definitions for execution traces and trace equivalence.
 |*)
 
-CoInductive trace {E} :=
-| Cons (l : @label E) (s : trace)
+CoInductive trace {E R} :=
+| Cons (l : @label E R) (s : trace)
 | Nil.
 
 Program Definition htr {E C X} :
-  mon (@trace E -> ctree E C X -> Prop) :=
+  mon (@trace E X -> ctree E C X -> Prop) :=
   {| body R s t :=
     match s with
-    | Cons l s' => exists t', trans l t t' /\ R s' t'
+    (* TODO : Active or passive? *)
+    | Cons l s' => exists t', trans l t (Active t') /\ R s' t'
     | Nil => True
     end
   |}.
@@ -32,12 +33,12 @@ Defined.
 
 Definition has_trace {E C X} := gfp (@htr E C X).
 
-Definition tracincl {E C D X Y}
-  (t : ctree E C X) (t' : ctree E D Y) :=
+Definition tracincl {E C D X}
+  (t : ctree E C X) (t' : ctree E D X) :=
   forall s, has_trace s t -> has_trace s t'.
 
-Definition traceq {E C D X Y}
-  (t : ctree E C X) (t' : ctree E D Y) :=
+Definition traceq {E C D X}
+  (t : ctree E C X) (t' : ctree E D X) :=
   tracincl t t' /\ tracincl t' t.
 
 (*|
@@ -68,18 +69,28 @@ Tactic Notation "__trace_play" "in" hyp(H) :=
   rewrite ctree_eta in TR; cbn in TR;
   inv_trans; subst.
 
+(* Lemma ss_proper_trans :  *)
+
 (*|
 Trace inclusion is weaker than similarity,
 and trace equivalence is weaker than bisimilarity.
 |*)
 Lemma ssim_tracincl : forall {E C X} (t t' : ctree E C X),
-  ssim eq t t' -> tracincl t t'.
+ssim Leq t t' -> tracincl t t'.
 Proof.
-  red. red. intros. revert t t' H s H0. coinduction R CH. intros.
+  red. red. intros. 
+  revert t t' H s H0. coinduction R CH. intros.
   simpl. destruct s; auto.
+  (* Unset Printing Notations.  *)
   step in H0. cbn in H0. destruct H0 as (? & ? & ?).
   step in H. apply H in H0. destruct H0 as (? & ? & ? & ? & ?). subst.
-  exists x1. split. apply H0. eapply CH. apply H2. red. apply H1.
+  inv H0; try easy. 
+  exists x. split. 
+  2: eapply CH; eauto.
+  (* Print transR.  *)
+  unfold Leq in H3. assert (eq l x0). 
+  erewrite (ActAct) with (t:=x). 
+  rewrite H2. apply H0. eapply CH. apply H2. red. apply H1.
 Qed.
 
 Lemma sbisim_traceq : forall {E C X} (t t' : ctree E C X),
